Dpda/RepeatBindMap.lean
@@ -4,6 +4,19 @@ import Mathlib.Data.Fintype.Basic
 import Mathlib.Data.Fintype.Prod
 import Mathlib.Data.Fintype.Option
 
+lemma repeat_succ_outer {α} (f : α → α) (n : ℕ) (a : α) :
+  Nat.repeat f (n + 1) a = f (Nat.repeat f n a) := by rfl
+
+lemma repeat_succ_inner {α} (f : α → α) (n : ℕ) (a : α) :
+  Nat.repeat f (n + 1) a = Nat.repeat f n (f a) := by
+   induction n with
+   | zero => rfl
+   | succ d hd =>
+      rw [repeat_succ_outer]
+      nth_rw 2 [repeat_succ_outer]
+      apply congr_arg
+      exact hd
+
 lemma repeat_bind_map2 {m} [Monad m] [LawfulMonad m] α β
   (α2β : α → β)
   (mfα : α → m α)
